

$$A(z) B(w) = \sum_{n=-\infty}^{\infty} \frac{(AB)_n(w)}{(z-w)^{n+1}}$$

We recall that

$$[A[B]_n]_m = (-1)^{ab} [B[A]_m]_n + \sum_{j=0}^{m-1} \binom{m-1}{j} ([AB]_{m-j})_n + j \quad m \geq 1$$

$$\text{Let } A=T \quad B=V_1 \quad C=V_2$$

$$[TV_1]_2 = V_1 \quad [TV_2]_2 = V_2$$

$$[TV_1]_1 = \partial V_1 \quad [TV_2]_1 = \partial V_2$$

We need to check

$$m > 2 \Rightarrow [T[V_1 V_2]_1]_m = 0$$

$$m = 2 \Rightarrow [T[V_1 V_2]_1]_m = [V_1 V_2]_1$$

$$m = 1 \Rightarrow [T[V_1 V_2]_1]_m = \partial[V_1 V_2]_1$$

$$\begin{aligned} & n=1 \\ \Rightarrow [T[V_1 V_2]_1]_m &= [V_1 [TV_2]_m]_1 + \sum_{j=0}^{m-1} \binom{m-1}{j} ([TV_1]_{m-j} V_2)_{1+j} \end{aligned}$$

When  $m > 2$

$$[T[V_1 V_2]_1]_m = \underbrace{[V_1 \quad 0]_1}_0 + (m-1) [TV_1]_2 V_2]_{m-1} + [TV_1]_1 V_2]_m$$

$$= 0 + (m-1) [V_1 V_2]_{m-1} + [\partial V_1 V_2]_m$$

$$= (m-1) [V_1 V_2]_{m-1} + (1-m) [V_1 V_2]_{m-1}$$

$$= 0$$

$$\text{But } [\partial AB]_n = (1-n) [AB]_{n-1}$$

When  $m=2$

$$[T[V_1 V_2]_1]_2 = [V_1 [TV_2]_2]_1 + [[TV_1]_2 V_2]_1 + [[TV_1]_1 V_2]_2$$

$$= [V_1 V_2]_1 + [V_1 V_2]_1 + [\partial V_1 V_2]_2$$

$$= 2[V_1 V_2]_1 - [V_1 V_2]_1 = [V_1 V_2]_1$$

When  $m=1$

$$[T[V_1 V_2]_1]_1 = [V_1 [TV_2]_1]_1 + [[TV_1]_1 V_2]_1$$

$$= [V_1 \partial V_2]_1 + [\partial V_1 V_2]_1$$

$$= \partial [V_1 V_2]_1 \quad \square$$

$\Rightarrow [V_1 V_2]_1$  is Primary and conformal dimension 1.